Add deadline parameter to MathBounty contract

examples/math-bounty/src-hs/MathBounty.hs
@@ -1,15 +1,45 @@
+{-# OPTIONS_GHC -cpp -XMagicHash #-}
+{- For Hugs, use the option -F"cpp -P -traditional" -}
+
 module MathBounty where
 
 import qualified Prelude
+import qualified PlutusLedgerApi_V1_Interval
+import qualified PlutusLedgerApi_V1_Time
 import qualified PlutusLedgerApi_V3_Contexts
+import qualified PlutusTx_Enum
+import qualified PlutusTx_Eq
+import qualified PlutusTx_Functor
+import qualified PlutusTx_Ord
+
+#ifdef __GLASGOW_HASKELL__
+import qualified GHC.Base
+#else
+-- HUGS
+import qualified IOExts
+#endif
+
+#ifdef __GLASGOW_HASKELL__
+unsafeCoerce :: a -> b
+unsafeCoerce = GHC.Base.unsafeCoerce#
+#else
+-- HUGS
+unsafeCoerce :: a -> b
+unsafeCoerce = IOExts.unsafeCoerce
+#endif
 
 data Datum =
-   MkDatum Prelude.Integer
+   MkDatum Prelude.Integer PlutusLedgerApi_V1_Time.POSIXTime
 
 square :: Datum -> Prelude.Integer
 square d =
   case d of {
-   MkDatum square0 -> square0}
+   MkDatum square0 _ -> square0}
+
+deadline :: Datum -> PlutusLedgerApi_V1_Time.POSIXTime
+deadline d =
+  case d of {
+   MkDatum _ deadline0 -> deadline0}
 
 data Redeemer =
    MkRedeemer Prelude.Integer
@@ -21,6 +51,32 @@ guess r =
 
 mathBounty :: Datum -> Redeemer -> PlutusLedgerApi_V3_Contexts.ScriptContext
               -> Prelude.Bool
-mathBounty datum redeemer _ =
-  (Prelude.==) ((Prelude.*) (guess redeemer) (guess redeemer)) (square datum)
+mathBounty datum redeemer ctx =
+  let {
+   guessCorrect = let {guess0 = guess redeemer} in
+                  (PlutusTx.Eq.==) ((PlutusTx.Numeric.*) guess0 guess0)
+                    (square datum)}
+  in
+  let {
+   beforeDeadline = let {
+                     deadlineRange = PlutusLedgerApi_V1_Interval.to
+                                       (PlutusLedgerApi_V1_Time.getPOSIXTime
+                                         (deadline datum))}
+                    in
+                    let {
+                     txRange = PlutusTx_Functor.fmap
+                                 (unsafeCoerce (\_ ->
+                                   PlutusLedgerApi_V1_Interval.coq_Functor__Interval))
+                                 PlutusLedgerApi_V1_Time.getPOSIXTime
+                                 (PlutusLedgerApi_V3_Contexts.txInfoValidRange
+                                   (PlutusLedgerApi_V3_Contexts.scriptContextTxInfo
+                                     ctx))}
+                    in
+                    PlutusLedgerApi_V1_Interval.contains
+                      (unsafeCoerce (\_ -> PlutusTx_Enum.coq_Enum__Z))
+                      (unsafeCoerce (\_ -> PlutusTx_Eq.coq_Eq__Z))
+                      (unsafeCoerce (\_ -> PlutusTx_Ord.coq_Ord__Z))
+                      (unsafeCoerce deadlineRange) txRange}
+  in
+  (Prelude.&&) guessCorrect beforeDeadline
 
