examples/math-bounty/src-hs/MathBountyFixed.hs
@@ -1,40 +1,67 @@
 module MathBountyFixed where
 
 import qualified Prelude
+import qualified PlutusLedgerApi.V1.Interval
+import qualified PlutusLedgerApi.V1.Time
 import qualified PlutusLedgerApi.V3.Contexts
+import qualified PlutusTx.Functor
+import qualified PlutusTx.Eq
+import qualified PlutusTx.Numeric
 
 import PlutusTx
 import PlutusTx.Prelude qualified as PlutusTx
 import PlutusTx.Show qualified as PlutusTx
 
 data Datum =
-   MkDatum Prelude.Integer
+  MkDatum Prelude.Integer PlutusLedgerApi.V1.Time.POSIXTime
 
 PlutusTx.unstableMakeIsData ''Datum
 
+{-# INLINEABLE square #-}
 square :: Datum -> Prelude.Integer
 square d =
-  case d of {
-   MkDatum square0 -> square0}
-{-# INLINEABLE square #-}
+  case d of
+    MkDatum square0 _ -> square0
+
+{-# INLINEABLE deadline #-}
+deadline :: Datum -> PlutusLedgerApi.V1.Time.POSIXTime
+deadline d =
+  case d of
+    MkDatum _ deadline0 -> deadline0
 
 data Redeemer =
-   MkRedeemer Prelude.Integer
+  MkRedeemer Prelude.Integer
 
 PlutusTx.unstableMakeIsData ''Redeemer
 
+{-# INLINEABLE guess #-}
 guess :: Redeemer -> Prelude.Integer
 guess r =
-  case r of {
-   MkRedeemer guess0 -> guess0}
-{-# INLINEABLE guess #-}
+  case r of
+    MkRedeemer guess0 -> guess0
 
-mathBounty :: Datum -> Redeemer -> PlutusLedgerApi.V3.Contexts.ScriptContext
-              -> Prelude.Bool
-mathBounty datum redeemer _ =
-  (Prelude.==) ((Prelude.*) (guess redeemer) (guess redeemer)) (square datum)
 {-# INLINEABLE mathBounty #-}
+mathBounty :: Datum -> Redeemer -> PlutusLedgerApi.V3.Contexts.ScriptContext -> Prelude.Bool
+mathBounty datum redeemer ctx =
+  let
+    guessCorrect =
+      let guess0 = guess redeemer in
+        (PlutusTx.Eq.==) ((PlutusTx.Numeric.*) guess0 guess0) (square datum)
 
+    beforeDeadline =
+      let
+        deadlineRange =
+          PlutusLedgerApi.V1.Interval.to (PlutusLedgerApi.V1.Time.getPOSIXTime (deadline datum))
+
+        txRange =
+          PlutusTx.Functor.fmap PlutusLedgerApi.V1.Time.getPOSIXTime
+            (PlutusLedgerApi.V3.Contexts.txInfoValidRange (PlutusLedgerApi.V3.Contexts.scriptContextTxInfo ctx))
+      in
+      PlutusLedgerApi.V1.Interval.contains deadlineRange txRange
+  in
+  (Prelude.&&) guessCorrect beforeDeadline
+
+{-# INLINEABLE mathBountyUntypedValidator #-}
 mathBountyUntypedValidator :: BuiltinData -> BuiltinData -> BuiltinData -> ()
 mathBountyUntypedValidator datum redeemer ctx =
   PlutusTx.check
@@ -43,7 +70,6 @@ mathBountyUntypedValidator datum redeemer ctx =
     (PlutusTx.unsafeFromBuiltinData redeemer)
     (PlutusTx.unsafeFromBuiltinData ctx)
   )
-{-# INLINEABLE mathBountyUntypedValidator #-}
 
 mathBountyValidatorScript :: CompiledCode (BuiltinData -> BuiltinData -> BuiltinData -> ())
 mathBountyValidatorScript = $$(PlutusTx.compile [|| mathBountyUntypedValidator ||])
