examples/math-bounty/src-coq/MathBounty.v
@@ -22,7 +22,9 @@ Import GHC.Base.Notations.
 
 Require PlutusTx_Bool.
 Require Import ZArith.BinInt.
+Require Import PlutusTx_Eq.
 Require Import PlutusTx_Functor.
+Require Import PlutusTx_Numeric.
 Require Import PlutusLedgerApi_V1_Time.
 Require Import PlutusLedgerApi_V1_Interval.
 Require Import PlutusLedgerApi_V3_Contexts.
@@ -31,33 +33,35 @@ Require Import PlutusLedgerApi_V3_Contexts.
   A very simple Math Bounty smart contract.
   Inspired by the math bounty example from https://github.com/ernius/plutus-cardano-samples
 
-  The contract stores a square number in the Datum, which can be redeemed by guessing the square root of the number.
+  The contract stores a square number in the Datum, which can be redeemed by guessing the square root of the number,
+  but only before the deadline passes.
 *)
 
-Record Datum := MkDatum { square : Z }.
+Record Datum := MkDatum { square : Z; deadline : POSIXTime }.
 Record Redeemer := MkRedeemer { guess : Z }.
 
 Definition mathBounty : Datum -> Redeemer -> ScriptContext -> bool :=
-  fun datum redeemer ctx => (guess redeemer * guess redeemer =? square datum)%Z.
+  fun datum redeemer ctx =>
+    let guessCorrect :=
+      let guess := guess redeemer in
+      (guess * guess =? square datum)%Z in
+    let beforeDeadline :=
+      let deadlineRange := to (getPOSIXTime (deadline datum)) in
+      let txRange := fmap getPOSIXTime (txInfoValidRange (scriptContextTxInfo ctx)) in
+      contains deadlineRange txRange
+    in
+    (guessCorrect && beforeDeadline)%bool.
 
-Theorem mathBountyCorrect : forall datum redeemer ctx, mathBounty datum redeemer ctx = true -> (guess redeemer * guess redeemer = square datum)%Z.
+Theorem mathBounty_guessCorrect : forall datum redeemer ctx, (mathBounty datum redeemer ctx = true) -> (guess redeemer * guess redeemer)%Z = square datum.
 Proof.
   intros datum redeemer ctx H.
   unfold mathBounty in H.
-  apply Z.eqb_eq in H.
-  exact H.
+  apply Bool.andb_true_iff in H.
+  destruct H as [H1 H2].
+  apply Z.eqb_eq in H1.
+  exact H1.
 Qed.
 
-Extract Inlined Constant Z.eqb => "(Prelude.==)".
-
-(*
-Timed version, which additionally checks that the guess is made before a deadline.
-Doesn't work, because hs-to-coq does not properly translate `deriving` clauses,
-so the `PlutusTx.Enum.Enum POSIXTime` instance is missing.
-
-Definition timedMathBounty : Datum -> Redeemer -> ScriptContext -> bool :=
-  fun datum redeemer ctx =>
-    let guessCorrect := (guess redeemer * guess redeemer =? square datum)%Z in
-    let beforeDeadline := contains (to (getPOSIXTime (deadline datum))) (fmap getPOSIXTime (txInfoValidRange (scriptContextTxInfo ctx))) in
-    andb guessCorrect beforeDeadline.
-*)
+Theorem mathBounty_guessCorrect_beforeDeadline : forall datum redeemer ctx, (mathBounty datum redeemer ctx = true) -> (guess redeemer * guess redeemer)%Z = square datum /\ contains (to (getPOSIXTime (deadline datum))) (fmap getPOSIXTime (txInfoValidRange (scriptContextTxInfo ctx))) = true.
+Proof.
+Admitted.
