examples/math-bounty/src-coq/ExtractionWrapper.v
@@ -8,5 +8,10 @@ Extraction Language Haskell.
 Unset Extraction Optimize.
 Set Extraction KeepSingleton.
 
+Require Import ZArith.BinInt.
+
+Extract Inlined Constant Z.eqb => "(PlutusTx.Eq.==)".
+Extract Inlined Constant Z.mul => "(PlutusTx.Numeric.*)".
+
 Require MathBounty.
 Extraction Library MathBounty.
