examples/math-bounty/README.md
@@ -4,8 +4,10 @@ This directory contains a simple Math Bounty smart contract, written in Coq usin
 
 The most interesting file is the contract script itself, [MathBounty.v](src-coq/MathBounty.v), which contains the `mathBounty` validator definition, as well as a proof of correctness.
 
-The [compile.sh](compile.sh) script can be used to compile the contract and extract it to Haskell, generating [MathBounty.hs](src-hs/MathBounty.hs). However, this extracted file needs some manual adjustments to be compilable by Plutus. The fixed file is available as [MathBountyFixed.hs](src-hs/MathBountyFixed.hs).
+The [extract.sh](extract.sh) script can be used to compile the contract and extract it to Haskell, generating [MathBounty.hs](src-hs/MathBounty.hs). (Before this step, make sure the translated Plutus Coq files are compiled by running `./scripts/compile.sh`)
 
-Finally, this fixed-up module can be compiled by running `cabal build math-bounty`, using the wrapper Cabal module defined in [math-bounty.cabal](math-bounty.cabal).
+However, this extracted file needs some manual adjustments to be compilable by Plutus. The fixed-up version is available as [MathBountyFixed.hs](src-hs/MathBountyFixed.hs).
 
-Note: The Cabal project doesn't actually compile, as the PlutusTx Plugin (which is required to compile Haskell to Plutus Core) only compiles with GHC 9.2 and above, and this project uses GHC 8.10.7 (this is the latest version supported by `hs-to-coq`).
+Finally, this fixed-up module can be compiled by running `cabal build --with-compiler=ghc-9.2 math-bounty`, using the wrapper Cabal project defined in [math-bounty.cabal](math-bounty.cabal).
+
+Note: It's required to compile the Cabal project with GHC >=9.2, as the PlutusTx Plugin (which is required to compile Haskell to Plutus Core) requires GHC >=9.2.
